\begin{center}
    $a_n = a_{n-1} + 2a_{n-2} \hspace{5ex} \forall n \geq 3, n \in \mathbb{N}$
\end{center}

Use induction to prove $a_n = 3(2^{n-1}) + 2(-1)^{n}$ for all $n$ if $a_1 = 1$ and $a_2 = 8$.

% \input{body.tex}

In order to construct a proof by induction we will demonstrate that the proposition holds for $a_1$ and $a_2$. By substituting in values of $1$ and $2$ into the formula $3(2^{n-1}) + 2(-1)^{n}$ we produce the following results.

\begin{center}
    $3(2^{1-1}) + 2(-1)^{1} = 1 = a_1$ \\
    $3(2^{2-1}) + 2(-1)^{2} = 8 = a_2$
\end{center}

This shows that the proposition $P(n) := a_n = 3(2^{n-1}) + 2(-1)^{n}$ is true for $P(1), P(2)$. We will now assume that the proposition holds for $P(n-1), P(n-2)$ and manupulate the initial recursive definition. Observe:

% $ a_3 = 8 + 2 \cdot 1 = 10 $ \\
% $ a_3 = 3(2^{2}) + 2(-1)^{3} = 10 $ \\
\begin{center}
\begin{tabular}{lcl}
    $ a_n = a_{n-1} + 2a_{n-2} $ & $\iff$ \\
    $ a_n = 3(2^{n-2}) + 2(-1^{n-1}) + 2(3(2^{n-3})) + 2(-1)^{n-2} $ & $\iff$ & $\star$ \\
    $ a_n = 3(2^{n-2}) + 6(2^{n-3}) + 2(-1^{n-3}) + 4(-1)^{n-2} $ & $\iff$ & Distribute and rearrange terms\\
    $ a_n = 3(2^{n-2} + 2 \cdot 2^{n-3}) + 2((-1)^{n-1}) + 2(-1)^{n-2})$  & $\iff$ & Extract common factors\\
    $ a_n = 3(2^{n-2} + 2^{n-2}) + 2((1)(-1)^{n-1} + (-1)(2)(-1)^{n-1})$  & $\iff$ & Re-represent to match exponents\\
    $ a_n = 3(2)2^{n-2} + 2(-1)(-1)^{n-1} $  & $\iff$ & Simplify like terms\\
    $ a_n = 3(2^{n-1}) + 2(-1)^{n} $  & $\iff$ & Simplify\\
\end{tabular}
\end{center}


The result of the above work is that $ a_n = 3(2^{n-1}) + 2(-1)^{n} $. We achieved this after assuming that $P(n-1), P(n-2)$ both were true. This inductive step is applied on the line denoted with a $\star$. This means that by knowing $P(1), P(2)$ to both be true (as verified earlier) we can determine $P(3)$ to be true and so forth. 

Therefore $a_n = 3(2^{n-1}) + 2(-1)^{n}$ for all positive integers $n$.

Q.E.D